Created unif_function.v. Started refactoring unif.v to use substitutions in `list (var * btree)` form rather than functions. Renamed unifies to unifiesb in unif_function.v as it is defined using booleans, and renamed consequent lemmas accordingly.

theories/core/unif_function.v
@@ -5,9 +5,6 @@ From mathcomp Require Import finmap.
 Require Import preamble hierarchy monad_lib fail_lib state_lib.
 From HB Require Import structures.
 
-Require Import List.
-Import ListNotations.
-
 Set Implicit Arguments.
 Unset Strict Implicit.
 Unset Printing Implicit Defensive.
@@ -234,19 +231,25 @@ Lemma btree_eq_boolP : Equality.axiom btree_eq_dec.
 Proof. move=> x y. case: btree_eq_dec => //= H; by constructor. Qed.
 HB.instance Definition _ := hasDecEq.Build _ btree_eq_boolP.
 
-Definition substType : UU0 := list (var * btree).
+Definition substType : UU0 := var -> btree.
+
+Definition subst0 : substType := btVar.
+
+Definition subst1 (x : var) (t : btree) (v : var) : btree :=
+  if v == x then t else btVar v.
 
 (* t[x\u] *)
-Fixpoint subst x u t : btree :=
+Fixpoint subst (s : var -> btree) t : btree :=
 match t with
-| btVar v => if (x == v) then u else t
+| btVar v => s v
 | btInt _ => t
-| btNode t1 t2 => btNode (subst x u t1) (subst x u t2)
+| btNode t1 t2 => btNode (subst s t1) (subst s t2)
 end.
 
-Definition subst_list (s : substType) t : btree :=
-  foldl (fun t (p : var * btree)  => subst p.1 p.2 t) t s.
+Definition subst_comp (s1 s2 : var -> btree) (v : var) : btree :=
+  subst s2 (s1 v).
 
+Definition subst_rul := (var * btree)%type.
 Definition constr := (btree * btree)%type.
 Definition constr_list := list constr.
 
@@ -264,10 +267,8 @@ Fixpoint vars (t : btree) : list var :=
   | btNode t1 t2 => union (vars t1) (vars t2)
   end.
 
-(*
-
-Definition unifies v u t1 t2 := subst sm t1 == subst sm t2.
-Definition unifies_pairs (sm : substType) := all (fun p => unifies sm p.1 p.2).
+Definition unifiesb (sm : substType) t1 t2 := subst sm t1 == subst sm t2.
+Definition unifiesb_pairs (sm : substType) := all (fun p => unifiesb sm p.1 p.2).
 
 Fixpoint size_tree (t : btree) : nat :=
   if t is btNode t1 t2 then 1 + size_tree t1 + size_tree t2 else 1.
@@ -381,29 +382,29 @@ Qed.
 Lemma substD : {morph subst: s1 s2 / subst_comp s1 s2 >-> s2 \o s1}.
 Proof. by move=> s1 s2; apply: boolp.funext; elim => //= t1 -> t2 ->. Qed.
 
-Lemma unifies_same sm t : unifies sm t t.
-Proof. by rewrite /unifies. Qed.
+Lemma unifiesb_same sm t : unifiesb sm t t.
+Proof. by rewrite /unifiesb. Qed.
 
-Lemma unifies_pairs_same sm t l :
-  unifies_pairs sm l -> unifies_pairs sm ((t,t) :: l).
+Lemma unifiesb_pairs_same sm t l :
+  unifiesb_pairs sm l -> unifiesb_pairs sm ((t,t) :: l).
 Proof.
   move=> H; apply /andP; split => //.
-  exact: unifies_same.
+  exact: unifiesb_same.
 Qed.
 
-Lemma unifies_swap sm t1 t2 :
-  unifies sm t1 t2 = unifies sm t2 t1.
-Proof. by rewrite /unifies eq_sym. Qed.
+Lemma unifiesb_swap sm t1 t2 :
+  unifiesb sm t1 t2 = unifiesb sm t2 t1.
+Proof. by rewrite /unifiesb eq_sym. Qed.
 
-Lemma unifies_pairs_swap sm t1 t2 l :
-  unifies_pairs sm ((t1, t2) :: l) = unifies_pairs sm ((t2, t1) :: l).
-Proof. elim: l => /= [ | a l IH ]; by rewrite unifies_swap. Qed.
+Lemma unifiesb_pairs_swap sm t1 t2 l :
+  unifiesb_pairs sm ((t1, t2) :: l) = unifiesb_pairs sm ((t2, t1) :: l).
+Proof. elim: l => /= [ | a l IH ]; by rewrite unifiesb_swap. Qed.
 
-Definition unifiesP (sm : substType) t1 t2 := subst sm t1 = subst sm t2.
-Definition unifiesP_pairs (sm : substType) (l : constr_list) :=
-  forall t1 t2, (t1,t2) \in l -> unifiesP sm t1 t2.
+Definition unifies (sm : substType) t1 t2 := subst sm t1 = subst sm t2.
+Definition unifies_pairs (sm : substType) (l : constr_list) :=
+  forall t1 t2, (t1,t2) \in l -> unifies sm t1 t2.
 
-Lemma unifP_pairs sm l : reflect (unifiesP_pairs sm l) (unifies_pairs sm l).
+Lemma unifb_pairs sm l : reflect (unifies_pairs sm l) (unifiesb_pairs sm l).
 Proof.
 apply/(iffP allP) => /= H.
 - by move=> t1 t2 Ht; apply/eqP/(H (t1,t2)).
@@ -460,29 +461,29 @@ Definition unify t1 t2 : N (unit * substType)%type :=
 
 Section Soundness.
 
-Lemma unifies_subst s v t :
-  v \notin vars t -> unifies (subst_comp (subst1 v t) s) (btVar v) t.
-Proof. by move=> ?; rewrite /unifies substD /= subst_same // /subst1 eqxx. Qed.
+Lemma unifiesb_subst s v t :
+  v \notin vars t -> unifiesb (subst_comp (subst1 v t) s) (btVar v) t.
+Proof. by move=> ?; rewrite /unifiesb substD /= subst_same // /subst1 eqxx. Qed.
 
-Lemma unifies_pairs_subst s v t l :
+Lemma unifiesb_pairs_subst s v t l :
   v \notin vars t ->
-  unifies (subst_comp (subst1 v t) s) (btVar v) t &&
-  unifies_pairs (subst_comp (subst1 v t) s) l =
-  unifies_pairs s ([seq subst_pair (subst1 v t) i | i <- l]).
+  unifiesb (subst_comp (subst1 v t) s) (btVar v) t &&
+  unifiesb_pairs (subst_comp (subst1 v t) s) l =
+  unifiesb_pairs s ([seq subst_pair (subst1 v t) i | i <- l]).
 Proof.
 move => nin; elim: l => /= [| a l IHl].
-- by rewrite unifies_subst.
-- by rewrite -IHl [RHS]andbCA !andbA /subst_comp /unifies /= !substD.
+- by rewrite unifiesb_subst.
+- by rewrite -IHl [RHS]andbCA !andbA /subst_comp /unifiesb /= !substD.
 Qed.
 
 Lemma unify_subst_sound h v t l :
   (forall l,
     runActionT (unify2 h l) >>=
-    assert (fun x => unifies_pairs x.2 l) =
+    assert (fun x => unifiesb_pairs x.2 l) =
     runActionT (unify2 h l)
   ) ->
   runActionT (unify_subst (unify2 h) v t l) >>= 
-    assert (fun x => unifies_pairs x.2 ((btVar v, t) :: l)) =
+    assert (fun x => unifiesb_pairs x.2 ((btVar v, t) :: l)) =
   runActionT (unify_subst (unify2 h) v t l).
 Proof.
 rewrite /unify_subst.
@@ -490,13 +491,13 @@ case/boolP: (v \in _) => Hocc // IH.
   by rewrite runActionTfail bindfailf.
 rewrite runActionTbind runActionTwrite !bindretf !bindA /= -[in RHS]IH.
 under eq_bind do rewrite bindretf /=.
-under eq_bind do rewrite assertE unifies_pairs_subst //.
+under eq_bind do rewrite assertE unifiesb_pairs_subst //.
 rewrite bindA.
 by under [in RHS]eq_bind do rewrite assertE bindA bindretf.
 Qed.
 
 Theorem unify2_sound h l :
-  runActionT (unify2 h l) >>= assert (fun x => unifies_pairs x.2 l) =
+  runActionT (unify2 h l) >>= assert (fun x => unifiesb_pairs x.2 l) =
   runActionT (unify2 h l).
 Proof.
 elim: h l => /= [l | h IH l].
@@ -509,24 +510,24 @@ elim: h' l => //= [l | h' IH' [| [t1 t2] l] /=].
 destruct t1, t2; try by rewrite runActionTfail bindfailf.
 - case: ifPn; move=> /eqP eq.
   + rewrite eq -[RHS]IH'.
-    by under eq_bind do rewrite assertE unifies_same //=.
+    by under eq_bind do rewrite assertE unifiesb_same //=.
   + exact/unify_subst_sound.
 - exact/unify_subst_sound.
 - exact/unify_subst_sound.
-- under eq_bind do rewrite assertE unifies_swap.
+- under eq_bind do rewrite assertE unifiesb_swap.
   exact/unify_subst_sound.
 - have []:= eqVneq n n0 => /= H; try by rewrite runActionTfail bindfailf.
-  by under eq_bind do rewrite assertE H unifies_same /=.
-- under eq_bind do rewrite assertE unifies_swap.
+  by under eq_bind do rewrite assertE H unifiesb_same /=.
+- under eq_bind do rewrite assertE unifiesb_swap.
   exact/unify_subst_sound.
-- by under eq_bind do rewrite assertE /unifies !subst_btNode eqb_btNode -andbA.
+- by under eq_bind do rewrite assertE /unifiesb !subst_btNode eqb_btNode -andbA.
 Qed.
 
 Corollary soundness t1 t2:
-  unify t1 t2 >>= assert (fun x => unifies x.2 t1 t2) = unify t1 t2.
+  unify t1 t2 >>= assert (fun x => unifiesb x.2 t1 t2) = unify t1 t2.
 Proof.
 rewrite /unify /=.
-have Huup: forall s t1 t2, unifies s t1 t2 = unifies_pairs s [:: (t1, t2)]
+have Huup: forall s t1 t2, unifiesb s t1 t2 = unifiesb_pairs s [:: (t1, t2)]
 by move => *; rewrite /= andbT.
 under eq_bind do rewrite assertE Huup.
 exact: unify2_sound.
@@ -536,10 +537,10 @@ End Soundness.
 
 Section Completeness.
 
-Lemma not_unifies_occur v t s :
-  btVar v != t -> v \in vars t -> ~unifies s (btVar v) t.
+Lemma not_unifiesb_occur v t s :
+  btVar v != t -> v \in vars t -> ~unifiesb s (btVar v) t.
 Proof.
-rewrite /unifies.
+rewrite /unifiesb.
 move=> vt Ht /eqP Hun.
 have Hs: size_tree (subst s (btVar v)) >= size_tree (subst s t) by rewrite Hun.
 elim: t {Hun} vt Ht Hs => //= [v' | t1 IH1 t2 IH2] vt.
@@ -560,10 +561,10 @@ elim: t {Hun} vt Ht Hs => //= [v' | t1 IH1 t2 IH2] vt.
   by rewrite addnAC leq_addl.
 Qed.
 
-Lemma unifies_extend s v t t' :
-  unifies s (btVar v) t -> unifies s (subst (subst1 v t) t') t'.
+Lemma unifiesb_extend s v t t' :
+  unifiesb s (btVar v) t -> unifiesb s (subst (subst1 v t) t') t'.
 Proof.
-  rewrite /unifies.
+  rewrite /unifiesb.
   elim: t' => //= [v' | t1 IH1 t2 IH2].
   - rewrite /subst1 => /eqP Heq.
     case: ifP => // /eqP ->.
@@ -574,47 +575,47 @@ Proof.
     move => /eqP -> /eqP -> //.
 Qed.
 
-Lemma unifies_pairs_extend s v t l :
-  unifies_pairs s ((btVar v, t) :: l) ->
-  unifies_pairs s (map (subst_pair (subst1 v t)) l).
+Lemma unifiesb_pairs_extend s v t l :
+  unifiesb_pairs s ((btVar v, t) :: l) ->
+  unifiesb_pairs s (map (subst_pair (subst1 v t)) l).
 Proof.
   move => /= /andP [h1 h2].
-  apply /unifP_pairs.
+  apply /unifb_pairs.
   move => t1 t2 /mapP /= [] [t3 t4] Hl [-> ->].
-  have Hv : unifies s (btVar v) t by apply h1.
+  have Hv : unifiesb s (btVar v) t by apply h1.
   apply/eqP.
-  have: unifies s (subst (subst1 v t) t3) t3 by apply:unifies_extend.
-  have: unifies s (subst (subst1 v t) t4) t4 by apply:unifies_extend.
-  rewrite /unifies => /eqP -> /eqP ->.
-  move/unifP_pairs in h2.
+  have: unifiesb s (subst (subst1 v t) t3) t3 by apply:unifiesb_extend.
+  have: unifiesb s (subst (subst1 v t) t4) t4 by apply:unifiesb_extend.
+  rewrite /unifiesb => /eqP -> /eqP ->.
+  move/unifb_pairs in h2.
   exact /eqP/h2/Hl.
 Qed.
 
-Lemma unifies_pairs_btNode s tl1 tl2 tr1 tr2 l :
-  unifies s (btNode tl1 tl2) (btNode tr1 tr2) ->
-  unifies_pairs s l ->
-  unifies_pairs s ((tl1,tr1)::(tl2,tr2)::l).
+Lemma unifiesb_pairs_btNode s tl1 tl2 tr1 tr2 l :
+  unifiesb s (btNode tl1 tl2) (btNode tr1 tr2) ->
+  unifiesb_pairs s l ->
+  unifiesb_pairs s ((tl1,tr1)::(tl2,tr2)::l).
 Proof.
-  rewrite /unifies !subst_btNode => /eqP /eq_btNode -[H1 H2] Hs.
-  apply/unifP_pairs => t3 t4.
+  rewrite /unifiesb !subst_btNode => /eqP /eq_btNode -[H1 H2] Hs.
+  apply/unifb_pairs => t3 t4.
   rewrite !inE.
   case/orP => [/eqP[-> ->] // |].
   case/orP => [/eqP[-> ->] // |].
-  by apply/unifP_pairs.
+  by apply/unifb_pairs.
 Qed.
 
 Definition moregen s s' :=
   exists s2, forall t, subst s' t = subst s2 (subst s t).
 
 Lemma moregen_extend s v t s1 :
-  unifies s (btVar v) t ->
+  unifiesb s (btVar v) t ->
   moregen s1 s ->
   moregen (subst_comp (subst1 v t) s1) s.
 Proof.
   move=> Hs [s2 Hs2].
   exists s2 => t' /=.
   rewrite /subst_comp substD -Hs2.
-  exact/esym/eqP/unifies_extend.
+  exact/esym/eqP/unifiesb_extend.
 Qed.
 
 Lemma subst_del x t t' :
@@ -701,7 +702,7 @@ Qed.
 
 Lemma unify_subst_complete s h v t l :
   (forall l,
-    h > size (vars_pairs l) -> unifies_pairs s l ->
+    h > size (vars_pairs l) -> unifiesb_pairs s l ->
     exists s1,
     (forall t' (f : substType -> substType),
     catch (
@@ -712,7 +713,7 @@ Lemma unify_subst_complete s h v t l :
     runActionT (unify2 h l) >>= fun x => Ret (Some (f x.2)))
     /\ moregen s1 s) ->
   h.+1 > size (vars_pairs ((btVar v, t) :: l)) ->
-  unifies_pairs s ((btVar v, t) :: l) ->
+  unifiesb_pairs s ((btVar v, t) :: l) ->
   btVar v != t ->
   exists s1,
   (forall t' (f : substType -> substType),
@@ -728,12 +729,12 @@ Proof.
   rewrite /unify_subst.
   case: ifPn => vt.
     move: Hs => /= /andP [Hs1 ?].
-    elim: (@not_unifies_occur v t s) => //.
+    elim: (@not_unifiesb_occur v t s) => //.
   case: (IHh (map (subst_pair (subst1 v t)) l)) => //.
       have Hhv := @vars_pairs_decrease v t l vt.
       apply (leq_trans Hhv).
       by rewrite -ltnS.
-    by apply: unifies_pairs_extend.
+    by apply: unifiesb_pairs_extend.
   move=> s1 [Hun Hmg].
   exists (subst_comp (subst1 v t) s1); split => [t' f|].
   rewrite runActionTbind runActionTwrite bindretf /= !bindA.
@@ -757,7 +758,7 @@ Qed.
 
 Theorem unify2_complete s h l :
   h > size (vars_pairs l) ->
-  unifies_pairs s l ->
+  unifiesb_pairs s l ->
   exists s1,
   (forall t (f : substType -> substType),
   catch (
@@ -798,26 +799,26 @@ Proof.
 - exact: unify_subst_complete.
   (* SymVar *)
 - apply unify_subst_complete => //.
-  by rewrite unifies_pairs_swap.
+  by rewrite unifiesb_pairs_swap.
   (* SymSym *)
 - move: Hs => /= /andP [Hs1 Hs2].
   elim eq: (n == n0).
     apply IH' => //.
       rewrite /size_pairs /= -!addnA !add1n ltnS in Hh'.
       exact: ltnW.
-  have: unifies s (btInt n) (btInt n0) by apply Hs1.
-  rewrite /unifies !subst_btInt => /eqP -[].
+  have: unifiesb s (btInt n) (btInt n0) by apply Hs1.
+  rewrite /unifiesb !subst_btInt => /eqP -[].
   by move: eq => /eqP.
   (* SymFork *)
-- have : unifies s (btInt n) (btNode t2_1 t2_2) by apply Hs.
-  by rewrite /unifies subst_btInt subst_btNode.
+- have : unifiesb s (btInt n) (btNode t2_1 t2_2) by apply Hs.
+  by rewrite /unifiesb subst_btInt subst_btNode.
   (* ForkVar *)
 - apply unify_subst_complete => //.
     by rewrite size_vars_pairs_swap.
-  by rewrite unifies_pairs_swap.
+  by rewrite unifiesb_pairs_swap.
   (* ForkSym *)
-- have : unifies s (btNode t1_1 t1_2) (btInt n) by apply Hs.
-  by rewrite /unifies subst_btInt subst_btNode.
+- have : unifiesb s (btNode t1_1 t1_2) (btInt n) by apply Hs.
+  by rewrite /unifiesb subst_btInt subst_btNode.
   (* ForkFork *)
 - apply: IH'.
       by rewrite -size_vars_pairs_btNode.
@@ -827,11 +828,11 @@ Proof.
     rewrite (addnAC (size_tree t1_1)) in Hh'.
     exact: ltnW.
   move: Hs => /andP [*].
-  exact: unifies_pairs_btNode.
+  exact: unifiesb_pairs_btNode.
 Qed.
 
 Corollary unify_complete s t1 t2 :
-  unifies s t1 t2 ->
+  unifiesb s t1 t2 ->
   exists s1,
   (forall t,
   catch (
@@ -850,176 +851,11 @@ have [s' [Hf Hmg]]: exists s1 : var -> btree, (forall t (f : substType -> substT
   moregen s1 s.
 apply unify2_complete.
 by rewrite addnC.
-by rewrite /unifies_pairs /all Hs.
+by rewrite /unifiesb_pairs /all Hs.
 exists s'; split => [t|//].
 exact: Hf(id).
 Qed.
 
-(*
-Lemma unify_subst_complete s h v t l :
-  (forall l,
-    h > size (vars_pairs l) -> unifies_pairs s l ->
-    exists s1,
-    (forall t',
-    catch (
-      runActionT (unify2 h l) >>=
-      assert (fun x => subst x.2 t' == subst s1 t') >>=
-      fun x => Ret (Some x.2)
-    ) (Ret None) =
-    runActionT (unify2 h l) >>= fun x => Ret (Some x.2))
-    /\ moregen s1 s) ->
-  h.+1 > size (vars_pairs ((btVar v, t) :: l)) ->
-  unifies_pairs s ((btVar v, t) :: l) ->
-  btVar v != t ->
-  exists s1,
-  (forall t',
-  catch (
-    runActionT (unify_subst (unify2 h) v t l) >>=
-    assert (fun x => subst x.2 t' == subst s1 t') >>=
-    fun x => Ret (Some x.2)
-  ) (Ret None) =
-  runActionT (unify_subst (unify2 h) v t l) >>= fun x => Ret (Some x.2))
-  /\ moregen s1 s.
-Proof.
-  move=> IHh Hh Hs Hv.
-  rewrite /unify_subst.
-  case: ifPn => vt.
-    move: Hs => /= /andP [Hs1 ?].
-    elim: (@not_unifies_occur v t s) => //.
-  case: (IHh (map (subst_pair (subst1 v t)) l)) => //.
-      have Hhv := @vars_pairs_decrease v t l vt.
-      apply (leq_trans Hhv).
-      by rewrite -ltnS.
-    by apply: unifies_pairs_extend.
-  move=> s1 [Hun Hmg].
-  exists (subst_comp (subst1 v t) s1); split => [t'|].
-  rewrite runActionTbind runActionTwrite bindretf /= !bindA.
-  under [RHS]eq_bind do rewrite bindretf => /=.
-  under eq_bind do rewrite bindretf.
-  have ->: forall m,
-    m >>= (fun x => Ret (Some (subst_comp (subst1 v t) x.2))) =
-    m >>= ((fun x =>
-            if x is Some x'
-            then Ret (Some (subst_comp (subst1 v t) x'))
-            else Ret None) \o
-           (fun x : unit * substType => Some x.2)).
-  by move => *; rewrite -bind_fmap.
-  have ->: forall m,
-    m >>= ((fun x =>
-            if x is Some x'
-            then Ret (Some (subst_comp (subst1 v t) x'))
-            else Ret None) \o
-           (fun x : unit * substType => Some x.2)) =
-    m >>= (fun x : unit * substType => Ret (Some x.2)) >>=
-    fun x => if x is Some x'
-            then Ret (Some (subst_comp (subst1 v t) x'))
-            else Ret None.
-  move => M' m; rewrite bindA.
-  by apply: eq_bind => x; rewrite bindretf.
-  rewrite -bindA -(Hun (subst (subst1 v t) t')) !bindA.
-  rewrite /assert /guard /=.
-  under eq_bind do rewrite !substD.
-  rewrite -!bindA.
-  admit.
-  apply moregen_extend => //.
-  by move: Hs => /andP [-> ?].
-Admitted.
-
-Theorem unify2_complete s h l :
-  h > size (vars_pairs l) ->
-  unifies_pairs s l ->
-  exists s1,
-  (forall t,
-  catch (
-    runActionT (unify2 h l) >>=
-    assert (fun x => subst x.2 t == subst s1 t) >>=
-    fun x => Ret (Some x.2)
-  ) (Ret None) =
-  runActionT (unify2 h l) >>= fun x => Ret (Some x.2))
-  /\ moregen s1 s.
-Proof.
-  elim: h l => //= h IH l Hh.
-  move Hh': (size_pairs l + 1) => h'.
-  have {Hh'} : h' > size_pairs l.
-    by rewrite -Hh' addn1 ltnS.
-  elim: h' l Hh => //= h' IH' [] //=.
-    move => *; exists subst0; split => // [t|].
-    by rewrite runActionTret !bindretf /assert eqxx bindskipf bindretf catchret.
-    exists s => t; by rewrite subst_zero.
-  case=> t1 t2 l Hh Hh' Hs.
-  destruct t1, t2 => /=.
-  (* VarVar *)
-- case: ifP => vv0.
-    move/eqP in vv0; subst v0.
-    apply IH'.
-    + apply/leq_trans: Hh.
-      rewrite ltnS.
-      exact: size_union2.
-    + rewrite /size_pairs /= -!addnA !add1n ltnS in Hh'.
-      exact: ltnW.
-    + move: Hs => /andP [? Hs]; apply Hs; by auto.
-  have Hvar : btVar v != btVar v0.
-    apply/negP => /eqP[] /eqP.
-    by rewrite vv0.
-  exact: unify_subst_complete.
-  (* VarSym *)
-- exact: unify_subst_complete.
-  (* VarFork *)
-- exact: unify_subst_complete.
-  (* SymVar *)
-- apply unify_subst_complete => //.
-  by rewrite unifies_pairs_swap.
-  (* SymSym *)
-- move: Hs => /= /andP [Hs1 Hs2].
-  elim eq: (n == n0).
-    apply IH' => //.
-      rewrite /size_pairs /= -!addnA !add1n ltnS in Hh'.
-      exact: ltnW.
-  have: unifies s (btInt n) (btInt n0) by apply Hs1.
-  rewrite /unifies !subst_btInt => /eqP -[].
-  by move: eq => /eqP.
-  (* SymFork *)
-- have : unifies s (btInt n) (btNode t2_1 t2_2) by apply Hs.
-  by rewrite /unifies subst_btInt subst_btNode.
-  (* ForkVar *)
-- apply unify_subst_complete => //.
-    by rewrite size_vars_pairs_swap.
-  by rewrite unifies_pairs_swap.
-  (* ForkSym *)
-- have : unifies s (btNode t1_1 t1_2) (btInt n) by apply Hs.
-  by rewrite /unifies subst_btInt subst_btNode.
-  (* ForkFork *)
-- apply: IH'.
-      by rewrite -size_vars_pairs_btNode.
-    rewrite /size_pairs /= in Hh' *.
-    rewrite !add1n !(addnS,addSn) in Hh'.
-    rewrite !addnA in Hh' *.
-    rewrite (addnAC (size_tree t1_1)) in Hh'.
-    exact: ltnW.
-  move: Hs => /andP [*].
-  exact: unifies_pairs_btNode.
-Qed.
-
-Corollary unify_complete s t1 t2 :
-  unifies s t1 t2 ->
-  exists s1,
-  (forall t,
-  catch (
-    unify t1 t2 >>=
-    assert (fun x => subst x.2 t == subst s1 t) >>=
-    fun x => Ret (Some x.2)
-  ) (Ret None) =
-  unify t1 t2 >>= fun x => Ret (Some x.2))
-  /\ moregen s1 s.
-Proof.
-rewrite /unify addnC => /eqP Hs.
-apply unify2_complete => //.
-apply/unifP_pairs => ? ?.
-by rewrite inE => /eqP[-> ->].
-Qed.
-*)
-
 End Completeness.
 
 End Unify.
-*)
